examples/crypto/acls-cap.fst
@@ -1,7 +1,20 @@
+(*--build-config
+    options:--z3timeout 10 --prims ../../lib/prims.fst --verify_module Pad --admit_fsi Seq --max_fuel 4 --initial_fuel 0 --max_ifuel 2 --initial_ifuel 1;
+    variables:LIB=../../lib;
+    other-files:$LIB/string.fst $LIB/list.fst
+            $LIB/ext.fst $LIB/classical.fst
+            $LIB/set.fsi $LIB/set.fst
+            $LIB/heap.fst $LIB/st.fst
+            $LIB/seq.fsi $LIB/seqproperties.fst
+            ../security/acls2.fst
+  --*)
+
+
 (* to be used with mac.fst and acls2.fst *)
 
 module Cap (* capabilities *)
-open Array
+open Seq
+open SeqProperties
 open ACLs2
 open MAC
 
