examples/crypto/rpc.fst
@@ -1,7 +1,22 @@
+(*--build-config
+    options:--z3timeout 10 --prims ../../lib/prims.fst --verify_module RPC --admit_fsi Seq --max_fuel 4 --initial_fuel 0 --max_ifuel 2 --initial_ifuel 1;
+    variables:LIB=../../lib;
+    other-files:$LIB/string.fst $LIB/list.fst
+            $LIB/ext.fst $LIB/classical.fst
+            $LIB/set.fsi $LIB/set.fst
+            $LIB/heap.fst $LIB/st.fst
+            $LIB/seq.fsi $LIB/seqproperties.fst
+            formatting.fst
+            sha1.fst
+            mac.fst
+  --*)
+
+
 (* Copyright (c) Microsoft Corporation.  All rights reserved.  *)
 
 module RPC
-open Array
+open Seq
+open SeqProperties
 open SHA1
 open Formatting
 open MAC
@@ -24,11 +39,11 @@ opaque logic type reqresp (msg:message) =
     (exists s.   msg = Formatting.request s    /\ Request s)
  \/ (exists s t. msg = Formatting.response s t /\ Response s t)
 
-let k = keygen reqresp 
+let k = keygen reqresp
 
 let client (s:string16) =
   assume (Request s);
-  send (append (utf8 s) (mac k (Formatting.request s))); 
+  send (append (utf8 s) (mac k (Formatting.request s)));
   recv (fun msg ->
     if length msg < macsize then failwith "Too short"
     else
@@ -42,17 +57,17 @@ let server () =
     if length msg < macsize then failwith "Too short"
     else
       let (v,m) = split msg (length msg - macsize) in
-      if length v > 65535 then failwith "Too long" 
+      if length v > 65535 then failwith "Too long"
       else
         let s = iutf8 v in
-        if verify k (Formatting.request s) m 
-        then  
+        if verify k (Formatting.request s) m
+        then
           ( assert (Request s);
             let t = "22" in
             assume (Response s t);
             send (append (utf8 t) (mac k (Formatting.response s t)))))
-  
-(* 
-let test () = 
-  server(); 
+
+(*
+let test () =
+  server();
   client "2 + 2? *)
