examples/crypto/sha1.fst
@@ -1,5 +1,14 @@
+(*--build-config
+    options:--z3timeout 10 --prims ../../lib/prims.fst --verify_module SHA1 --admit_fsi Seq --max_fuel 4 --initial_fuel 0 --max_ifuel 2 --initial_ifuel 1;
+    variables:LIB=../../lib;
+    other-files:$LIB/string.fst $LIB/list.fst
+            $LIB/ext.fst $LIB/classical.fst
+            $LIB/set.fsi $LIB/set.fst
+            $LIB/heap.fst $LIB/st.fst
+            $LIB/seq.fsi $LIB/seqproperties.fst
+  --*)
 module SHA1
-open Array
+open Seq
 
 type bytes = seq byte (* concrete byte arrays *)
 type text  = bytes    (* a type abbreviation, for clarity *)
